src/coq_formalism/utilities.v
@@ -1,0 +1,14 @@
+(***************************
+  Various Ltac code *)
+
+Ltac invc H := inversion H; clear H.  
+
+Ltac inv H := inversion H; subst.
+
+Ltac invsc H := inversion H; subst; clear H. 
+
+Ltac dest_sp H v := destruct H as [v]; intuition.
+
+Ltac destruct_all q2 q3 q' H1 := destruct H1 as [q2 H1];  destruct H1 as [q3 H1];  destruct H1 as [q']; intuition.
+
+Ltac exists_all q1 q2 q' := exists q1; exists q2; exists q'.
